Actually store balances in bank

src/Dafny/bank.dfy
@@ -1,22 +1,71 @@
 include "jrnl.s.dfy"
+include "int.dfy"
+include "marshal.dfy"
 
-const acct1: Addr := Addr(513, 0);
-const acct2: Addr := Addr(513, 8*8);
+const Acct1: Addr := Addr(513, 0);
+const Acct2: Addr := Addr(513, 8*8);
 
 /*
 Demo of bank transfer using axiomatized journal API
 */
 class Bank
 {
+    ghost const acct_sum: uint64;
+    ghost var acct1: uint64;
+    ghost var acct2: uint64;
+
     var jrnl: Jrnl;
+
+    static method encode_acct(x: uint64) returns (bs:seq<byte>)
+    modifies {}
+    ensures seq_encode([EncUInt64(x)]) == bs
+    {
+        var enc := new Encoder(8);
+        enc.EncInt(x);
+        bs := enc.FinishComplete();
+    }
+
+    static method decode_acct(bs:seq<byte>, ghost x: uint64) returns (x': uint64)
+    modifies {}
+    requires seq_encode([EncUInt64(x)]) == bs
+    ensures x' == x
+    {
+        var dec := new Decoder();
+        dec.Init(bs, [EncUInt64(x)]);
+        x' := dec.DecInt(x);
+    }
+
+    // NOTE: unused, but an example of how painful helper methods are
+    static method zeroAccount(jrnl: Jrnl, acct: Addr)
+    requires jrnl.Valid() ensures jrnl.Valid()
+    requires !jrnl.has_readbuf
+    requires jrnl.has_kind(acct, KindUInt64)
+    modifies jrnl
+    ensures !jrnl.has_readbuf
+    ensures jrnl.data == old(jrnl.data)[acct := seq_encode([EncUInt64(0)])]
+    {
+        var data := encode_acct(0);
+        jrnl.Write(acct, data);
+    }
+
     constructor()
     ensures this.Valid()
+    ensures acct1 == 100 && acct2 == 0
     {
         // BUG: we can't actually use the constant because then Dafny makes the type
         // of the map display expression map<int,int>.
-        assert 6 == KindUint64;
+        assert 6 == KindUInt64;
         var kinds: map<Blkno, Kind> := map[513:=6];
-        this.jrnl := new Jrnl(kinds);
+        var jrnl := new Jrnl(kinds);
+        var hundred_acct := encode_acct(100);
+        var zero_acct := encode_acct(0);
+        jrnl.Write(Acct1, hundred_acct);
+        jrnl.Write(Acct2, zero_acct);
+        this.jrnl := jrnl;
+
+        acct1 := 100;
+        acct2 := 0;
+        acct_sum := 100;
     }
 
     predicate Valid()
@@ -24,20 +73,45 @@ class Bank
     {
         && jrnl.Valid()
         && !jrnl.has_readbuf
-        && acct1 in jrnl.domain
-        && acct2 in jrnl.domain
-        && jrnl.size(acct1) == 64
-        && jrnl.size(acct2) == 64
+        && Acct1 in jrnl.domain
+        && Acct2 in jrnl.domain
+        && jrnl.size(Acct1) == 64
+        && jrnl.size(Acct2) == 64
+        && jrnl.data[Acct1] == seq_encode([EncUInt64(acct1)])
+        && jrnl.data[Acct2] == seq_encode([EncUInt64(acct2)])
+        && acct_sum == acct1 + acct2
     }
 
     // NOTE: this should be interpreted as the body of a transaction, which
     // needs to be surrounded with code to check for errors and abort
     method transfer()
     requires Valid() ensures Valid()
-    modifies jrnl
+    modifies {this,jrnl}
+    requires 0 < acct1
+    requires acct2+1 < 0x1_0000_0000_0000_000
+    ensures acct1 == old(acct1) - 1
+    ensures acct2 == old(acct2) + 1
     {
-        var x := jrnl.Read(acct1, 64);
-        x.Finish();
-        jrnl.Write(acct2, x.obj);
+        var x := jrnl.Read(Acct1, 64);
+        var acct1_val := decode_acct(x.obj, acct1);
+        x.obj := encode_acct(acct1_val-1);
+        x.SetDirty();
+        acct1 := acct1 - 1;
+
+        x := jrnl.Read(Acct2, 64);
+        var acct2_val := decode_acct(x.obj, acct2);
+        x.obj := encode_acct(acct2_val+1);
+        x.SetDirty();
+        acct2 := acct2 + 1;
+    }
+
+    // this is kind of silly but it gets the point across (without requiring the
+    // reader to understand Valid())
+    method audit() returns (b:bool)
+    modifies {}
+    requires Valid()
+    ensures b == (acct1 + acct2 == acct_sum)
+    {
+        return true;
     }
 }
